[WIP] [Dafny] Got rid of preconditions in a nasty way

compiler/dafny_new/translation/dafny_compilerProgScript.sml
@@ -8,53 +8,123 @@ open dafny_to_cakemlProgTheory
 open dafny_compilerTheory
 open cfTacticsLib  (* process_topdecs *)
 open dafny_transformProgTheory
+open fromSexpTheory  (* listsexp *)
+open stringTheory
+open numposrepTheory
+open simpleSexpTheory
+open ml_translatorTheory
+open simpleSexpParseTheory
+open dafny_compilerAProgTheory
 
 val _ = new_theory "dafny_compilerProg";
 
-val _ = translation_extends "dafny_transformProg";
+val _ = translation_extends "dafny_compilerAProg";
 
 val r = translate dafny_compilerTheory.dfy_to_cml_def;
 val r = translate dafny_compilerTheory.unpack_def;
 
-val r = translate fromSexpTheory.listsexp_def;
 
-val r = translate fromSexpTheory.locnsexp_def;
-val r = translate fromSexpTheory.locssexp_def;
-val r = translate stringTheory.isPrint_def;
-val r = translate numposrepTheory.n2l_def;  (* TODO precondition *)
-val r = translate ASCIInumbersTheory.n2s_def;  (* TODO precondition *)
-val r = translate ASCIInumbersTheory.HEX_def;  (* TODO precondition *)
-val r = translate ASCIInumbersTheory.num_to_hex_string_def;  (* TODO precondition *)
-val r = translate fromSexpTheory.encode_control_def;  (* TODO precondition *)
-val r = translate fromSexpTheory.SEXSTR_def;  (* TODO precondition *)
-val r = translate fromSexpTheory.litsexp_def;  (* TODO precondition *)
-val r = translate fromSexpTheory.optsexp_def;
-val r = translate fromSexpTheory.idsexp_def;  (* TODO precondition *)
-val r = translate fromSexpTheory.typesexp_def;  (* TODO precondition *)
-val r = translate fromSexpTheory.patsexp_def;  (* TODO precondition *)
-val r = translate fromSexpTheory.opsexp_def;  (* TODO precondition *)
-val r = translate fromSexpTheory.lopsexp_def;
-val r = translate fromSexpTheory.scsexp_def;
-val r = translate fromSexpTheory.expsexp_def;  (* TODO precondition *)
-val r = translate fromSexpTheory.type_defsexp_def;  (* TODO precondition *)
-val r = translate fromSexpTheory.decsexp_def;  (* TODO precondition *)
+(* --- *)
 
-val r = translate EL;  (* TODO precondition *)
-val r = translate simpleSexpParseTheory.strip_dot_def;
-val r = translate simpleSexpParseTheory.print_space_separated_def;
-val r = translate ASCIInumbersTheory.num_to_dec_string_def;  (* TODO precondition *)
-val r = translate simpleSexpParseTheory.escape_string_def;
-val r = translate simpleSexpParseTheory.print_sexp_def;  (* TODO precondition *)
+Triviality listsexp_alt:
+  listsexp = FOLDR (λs1 s2. SX_CONS s1 s2) nil
+Proof
+  rpt(CHANGED_TAC(CONV_TAC (DEPTH_CONV ETA_CONV))) >> simp[listsexp_def]
+QED
 
-val r = translate dafny_compilerTheory.cmlm_to_str_def;  (* TODO precondition *)
-val r = translate dafny_compilerTheory.main_function_def;  (* TODO precondition *)
+val _ = translate listsexp_alt;
+
+(* --- *)
+
+val _ = translate (fromSexpTheory.locnsexp_def |> SIMP_RULE list_ss []);  (* TODO is this necessary *)
+val _ = translate fromSexpTheory.locssexp_def;
+
+(* --- *)
+
+val _ = translate HEX_def
+
+Definition hex_alt_def:
+  hex_alt x = if x < 16 then HEX x else #"0"
+End
+
+val _ = translate hex_alt_def
+
+val _ = Q.prove(`!n. hex_alt_side n <=> T`,
+ PURE_REWRITE_TAC[fetch "-" "hex_alt_side_def",fetch "-" "hex_side_def"] >>
+ intLib.COOPER_TAC) |> update_precondition;
+
+Definition num_to_hex_string_alt:
+  num_to_hex_string_alt = n2s 16 hex_alt
+End
+
+Theorem num_to_hex_string_alt_intro:
+  !n. num_to_hex_string n = num_to_hex_string_alt n
+Proof
+  simp[num_to_hex_string_def,num_to_hex_string_alt,n2s_def] >>
+  ho_match_mp_tac COMPLETE_INDUCTION >>
+  rw[] >>
+  PURE_ONCE_REWRITE_TAC[numposrepTheory.n2l_def] >>
+  rw[hex_alt_def]
+QED
+
+val _ = translate numposrepTheory.n2l_def;
+
+val n2l_side_thm = Q.prove(`!n m. n2l_side n m <=> n <> 0`,
+  strip_tac >>
+  ho_match_mp_tac COMPLETE_INDUCTION >>
+  rpt strip_tac >>
+  PURE_ONCE_REWRITE_TAC[fetch "-" "n2l_side_def"] >>
+  rw[]) |> update_precondition
+
+val  _ = translate n2s_def;
+
+val n2s_side_thm = Q.prove(`!n f m. n2s_side n f m <=> n <> 0`,
+  rpt strip_tac >>
+  PURE_ONCE_REWRITE_TAC[fetch "-" "n2s_side_def"] >>
+  rw[n2l_side_thm]) |> update_precondition
+
+val _ = translate num_to_hex_string_alt;
+
+val _ = translate num_to_hex_string_alt_intro;
+
+(* --- *)
+
+val r = translate fromSexpTheory.encode_control_def;
+
+val _ = translate fromSexpTheory.SEXSTR_def;
+
+val _ = translate fromSexpTheory.litsexp_def;
+val litsexp_side_thm = Q.prove(`!v. litsexp_side v <=> T`,
+  PURE_ONCE_REWRITE_TAC[fetch "-" "litsexp_side_def"] >> rw[] >>
+                               intLib.COOPER_TAC) |> update_precondition
+
+val _ = translate optsexp_def;
+val _ = translate idsexp_def;
+val _ = translate typesexp_def;
+
+val _ = translate fromSexpTheory.patsexp_def;
+
+val _ = translate opsexp_def;
+val _ = translate lopsexp_def;
+val _ = translate scsexp_def;
+val _ = translate expsexp_def;
+
+val _ = translate type_defsexp_def;
+
+val _ = translate fromSexpTheory.decsexp_def;
+
+val r = translate dafny_compilerTheory.cmlm_to_str_def;
+
+val _ = ml_translatorLib.use_string_type true;
+
+val r = translate dafny_compilerTheory.main_function_def;
 
 val _ = type_of “main_function” = “:mlstring -> mlstring”
         orelse failwith "The main_function has the wrong type.";
 
-(* val _ = r |> hyp |> null orelse *)
-(*         failwith ("Unproved side condition in the translation of \ *)
-(*                   \dafny_compilerTheory.main_function_def"); *)
+val _ = r |> hyp |> null orelse
+        failwith ("Unproved side condition in the translation of \
+                  \dafny_compilerTheory.main_function_def");
 
 val main = process_topdecs
            ‘print (main_function (TextIO.inputAll TextIO.stdIn));’;
