compiler/dafny_new/translation/README.md
@@ -6,6 +6,9 @@ Translates CakeML's AST types, extending basisProg.
 [dafny_astProgScript.sml](dafny_astProgScript.sml):
 Translates Dafny's AST types.
 
+[dafny_compilerAProgScript.sml](dafny_compilerAProgScript.sml):
+TEST TEST TEST
+
 [dafny_compilerProgScript.sml](dafny_compilerProgScript.sml):
 Translates the Dafny to CakeML compiler.
 
